src/lang/Event.v
@@ -26,29 +26,34 @@ Module Ordering.
   (* TODO: support the SC atomics (#40) *)
   Inductive t :=
   | relaxed
-  | acquire
-  | release
-  | relacq
+  | acqrel
   | sc
   .
 
-  Definition le (lhs rhs:t): bool :=
-    match lhs, rhs with
-    | relaxed, _ => true
-    | _, relaxed => false
+  Inductive le: forall (lhs rhs:t), Prop :=
+  | le_relaxed_o o:
+      le relaxed o
+  | le_o_sc o:
+      le o sc
+  | le_acqrel_acqrel:
+      le acqrel acqrel
+  .
 
-    | _, sc => true
-    | sc, _ => false
+  Global Program Instance le_PreOrder: PreOrder le.
+  Next Obligation.
+    ii. destruct x; econs.
+  Qed.
+  Next Obligation.
+    ii. inv H; inv H0; econs.
+  Qed.
 
-    | _, relacq => true
-    | relacq, _ => false
-
-    | acquire, release => false
-    | acquire, acquire => true
-
-    | release, acquire => false
-    | release, release => true
-    end.
+  Definition le_dec (lhs rhs:t): {le lhs rhs} + {~ le lhs rhs}.
+  Proof.
+    destruct lhs, rhs;
+      (try by left; econs);
+      (try by right; intro X; inv X).
+  Defined.
+  Global Opaque le_dec.
 End Ordering.
 
 
@@ -56,42 +61,9 @@ Module MemEvent.
   Inductive t :=
   | read (loc:Loc.t) (val:Const.t) (ord:Ordering.t)
   | write (loc:Loc.t) (val:Const.t) (ord:Ordering.t)
-  | update (loc:Loc.t) (valr valw:Const.t) (ord:Ordering.t)
-  | fence (ord:Ordering.t)
+  | update (loc:Loc.t) (valr valw:Const.t) (ordr ordw:Ordering.t)
+  | fence (ordr ordw:Ordering.t)
   .
-
-  Definition is_writing (e:t): option (Loc.t * Const.t * Ordering.t) :=
-    match e with
-    | read _ _ _ => None
-    | write loc val ord => Some (loc, val, ord)
-    | update loc _ val ord => Some (loc, val, ord)
-    | fence _ => None
-    end.
-
-  Definition is_writing_to (loc:Loc.t) (e:t): option(Const.t * Ordering.t) :=
-    match is_writing e with
-    | None => None
-    | Some (loc', val, ord) =>
-      if Loc.eq_dec loc' loc
-      then Some (val, ord)
-      else None
-    end.
-
-  Definition is_reading (e:t): option (Loc.t * Const.t * Ordering.t) :=
-    match e with
-    | read loc val ord => Some (loc, val, ord)
-    | write _ _ _ => None
-    | update loc val _ ord => Some (loc, val, ord)
-    | fence _ => None
-    end.
-
-  Definition get_ordering (e:t): Ordering.t :=
-    match e with
-    | read _ _ ord => ord
-    | write _ _ ord => ord
-    | update _ _ _ ord => ord
-    | fence ord => ord
-    end.
 End MemEvent.
 
 
