src/opt/ReorderUpdate.v
@@ -26,46 +26,50 @@ Require Import Semantics.
 Set Implicit Arguments.
 
 
-Inductive reorder_update r1 l1 rmw1 o1: forall (i2:Instr.t), Prop :=
+Inductive reorder_update r1 l1 rmw1 or1 ow1: forall (i2:Instr.t), Prop :=
 | reorder_update_load
     r2 l2 o2
-    (ORD1: Ordering.le o1 Ordering.relaxed)
-    (ORD2: Ordering.le o2 Ordering.release)
+    (ORDR1: Ordering.le or1 Ordering.acqrel)
+    (ORDW1: Ordering.le ow1 Ordering.relaxed)
+    (ORD2: Ordering.le o2 Ordering.relaxed)
     (LOC: l1 <> l2)
-    (REGS: RegSet.disjoint (Instr.regs_of (Instr.update r1 l1 rmw1 o1))
+    (REGS: RegSet.disjoint (Instr.regs_of (Instr.update r1 l1 rmw1 or1 ow1))
                            (Instr.regs_of (Instr.load r2 l2 o2))):
-    reorder_update r1 l1 rmw1 o1 (Instr.load r2 l2 o2)
+    reorder_update r1 l1 rmw1 or1 ow1 (Instr.load r2 l2 o2)
 | reorder_update_store
     l2 v2 o2
-    (ORD1: Ordering.le o1 Ordering.relaxed)
+    (ORDR1: Ordering.le or1 Ordering.acqrel)
+    (ORDW1: Ordering.le ow1 Ordering.relaxed)
     (LOC: l1 <> l2)
-    (REGS: RegSet.disjoint (Instr.regs_of (Instr.update r1 l1 rmw1 o1))
+    (REGS: RegSet.disjoint (Instr.regs_of (Instr.update r1 l1 rmw1 or1 ow1))
                            (Instr.regs_of (Instr.store l2 v2 o2))):
-    reorder_update r1 l1 rmw1 o1 (Instr.store l2 v2 o2)
+    reorder_update r1 l1 rmw1 or1 ow1 (Instr.store l2 v2 o2)
 | reorder_update_update
-    r2 l2 rmw2 o2
-    (ORD1: Ordering.le o1 Ordering.relaxed)
-    (ORD2: Ordering.le o2 Ordering.release)
+    r2 l2 rmw2 or2 ow2
+    (ORDR1: Ordering.le or1 Ordering.acqrel)
+    (ORDW1: Ordering.le ow1 Ordering.relaxed)
+    (ORDR2: Ordering.le or2 Ordering.relaxed)
+    (ORDW2: Ordering.le ow2 Ordering.acqrel)
     (LOC: l1 <> l2)
-    (REGS: RegSet.disjoint (Instr.regs_of (Instr.update r1 l1 rmw1 o1))
-                           (Instr.regs_of (Instr.update r2 l2 rmw2 o2))):
-    reorder_update r1 l1 rmw1 o1 (Instr.update r2 l2 rmw2 o2)
+    (REGS: RegSet.disjoint (Instr.regs_of (Instr.update r1 l1 rmw1 or1 ow1))
+                           (Instr.regs_of (Instr.update r2 l2 rmw2 or2 ow2))):
+    reorder_update r1 l1 rmw1 or1 ow1 (Instr.update r2 l2 rmw2 or2 ow2)
 .
 
 Inductive sim_update: forall (st_src:lang.(Language.state)) (th_src:Local.t) (mem_k_src:Memory.t)
                         (st_tgt:lang.(Language.state)) (th_tgt:Local.t) (mem_k_tgt:Memory.t), Prop :=
 | sim_update_intro
-    r1 l1 from1 to1 vr1 vret1 vw1 releasedr1 releasedw1 rmw1 o1 i2
+    r1 l1 from1 to1 vr1 vret1 vw1 releasedr1 releasedw1 rmw1 or1 ow1 i2
     rs th1_src th1_tgt th2_src th3_src
     mem_k_src mem_k_tgt
-    (REORDER: reorder_update r1 l1 rmw1 o1 i2)
+    (REORDER: reorder_update r1 l1 rmw1 or1 ow1 i2)
     (RMW: RegFile.eval_rmw rs rmw1 vr1 = (vret1, vw1))
-    (READ: Local.read_step th1_src mem_k_src l1 from1 vr1 releasedr1 o1 th2_src)
-    (FULFILL: Local.fulfill_step th2_src mem_k_src l1 from1 to1 vw1 releasedw1 o1 th3_src)
+    (READ: Local.read_step th1_src mem_k_src l1 from1 vr1 releasedr1 or1 th2_src)
+    (FULFILL: Local.fulfill_step th2_src mem_k_src l1 from1 to1 vw1 releasedw1 ow1 th3_src)
     (RELEASED: Snapshot.le releasedr1 releasedw1)
     (LOCAL: sim_local th3_src th1_tgt):
     sim_update
-      (State.mk rs [Stmt.instr i2; Stmt.instr (Instr.update r1 l1 rmw1 o1)]) th1_src mem_k_src
+      (State.mk rs [Stmt.instr i2; Stmt.instr (Instr.update r1 l1 rmw1 or1 ow1)]) th1_src mem_k_src
       (State.mk (RegFun.add r1 vret1 rs) [Stmt.instr i2]) th1_tgt mem_k_tgt
 .
 
@@ -106,7 +110,6 @@ Proof.
       }
       i. des.
       exploit reorder_fulfill_read; try apply x3; try apply STEP_SRC; eauto.
-      { destruct o1; ss. }
       { eapply Local.read_step_future; eauto. }
       i. des.
       exploit reorder_read_read; try apply x0; try apply STEP1; eauto. i. des.
@@ -130,11 +133,10 @@ Proof.
       }
       i. des.
       exploit reorder_fulfill_write; try apply x3; try apply STEP_SRC; eauto.
-      { destruct o1; ss. }
       { eapply Local.read_step_future; eauto. }
       i. des.
       exploit reorder_read_write; try apply x0; try apply STEP1; eauto.
-      { destruct o1; ss. }
+      { i. rewrite ORDR1 in H0. inv H0. }
       i. des.
       eexists _, _, _, _, _, _. splits.
       * econs 2; [|econs 1]. econs 4; eauto. econs.
@@ -162,18 +164,16 @@ Proof.
       { eapply Local.read_step_future; eauto. }
       i. des.
       exploit reorder_fulfill_read; try apply x3; try apply STEP_SRC; eauto.
-      { destruct o1; ss. }
       { eapply Local.read_step_future; eauto. }
       i. des.
       exploit reorder_read_read; try apply x0; try apply STEP1; eauto. i. des.
       exploit reorder_fulfill_write; try apply STEP2; try apply STEP_SRC1; eauto.
-      { destruct o1; ss. }
       { eapply Local.read_step_future; eauto.
         eapply Local.read_step_future; eauto.
       }
       i. des.
       exploit reorder_read_write; try apply STEP3; try apply STEP4; eauto.
-      { destruct o1; ss. }
+      { i. rewrite ORDR1 in H0. inv H0. }
       { eapply Local.read_step_future; eauto. }
       i. des.
       eexists _, _, _, _, _, _. splits.
